implement bce protocol

bce/node.dfy
@@ -1,22 +1,127 @@
 module BCE_Protocol_Node {
 
+type symbol = nat
+type syndrome = seq<bool>
+
 datatype NodeState = Phase1 | Phase2 | Decided
+datatype Decision = Codeword | Bottom
 
 datatype Node = Node(
-    input: seq<nat>,
-    state: NodeState
+    f: nat,
+    n: nat,
+    id: nat,
+    codeword: seq<symbol>,      // my codeword
+    symbols: seq<symbol>,       // symbols[j] is the symbol sent by process j
+    decision: Decision,         
+    state: NodeState            // current state of the node
 )
 
-predicate Node_Init(s: Node)
+
+/****************************************************************************************/
+/*                                  PROTOCOL STEPS                                      */
+/****************************************************************************************/                 
+
+predicate nodeInit(s: Node, f:nat, n: nat, id: nat, my_codeword: seq<nat>)
+    requires n == 3*f + 1;
+    requires 0 <= id < n;
+    requires n == |my_codeword|;
 {
-    // TODO
-    true
+    && s.f == f
+    && s.n == n
+    && s.id == id
+    && s.codeword == my_codeword
+    && s.state == Phase1
 }
 
-predicate Node_Next(s:Node, s':Node)
+predicate receiveSymbols(s: Node, s':Node, received_symbols: seq<nat>) 
+    requires s.n == 3*s.f + 1;
+    requires s.state == Phase1;
+    requires 0 <= s.id < s.n;
+    requires s.n == |s.codeword|;
+    requires |received_symbols| == |s.codeword|;
+    requires received_symbols[s.id] == s.codeword[s.id];
 {
-    // TODO
-    true
+    s' == s.(
+        symbols := received_symbols,
+        state := Phase2)
 }
-    
+
+predicate receiveSyndromesAndDecide(s: Node, s': Node, syndromes: seq<syndrome>)
+    requires s.n == 3*s.f + 1;
+    requires s.state == Phase2;
+    requires 0 <= s.id < s.n;
+    requires s.n == |s.symbols| == |s.codeword|;
+    requires s.codeword[s.id] == s.symbols[s.id];
+    requires s.n == |syndromes|
+{   
+    if decideOnCodeWord(s, syndromes) then (
+        s' == s.(state := Decided,
+            decision := Codeword
+        )       
+    ) else (
+        s' == s.(state := Decided,  
+            decision := Bottom)
+    )
+}
+
+
+/****************************************************************************************/
+/*                             FUNCTIONS & PREDICATES                                   */
+/****************************************************************************************/ 
+
+
+/* Evaluates to true iff Node s should decide on its own codeword based on the 
+* BCE protocol */
+predicate decideOnCodeWord(s: Node, syndromes: seq<syndrome>) 
+    requires s.n == 3*s.f + 1;
+    requires s.state == Phase2;
+    requires 0 <= s.id < s.n;
+    requires s.n == |s.symbols| == |s.codeword|;
+    requires s.codeword[s.id] == s.symbols[s.id];
+    requires s.n == |syndromes|
+{
+    if countTrue(syndromes[s.id]) < s.n - s.f then (
+        false
+    ) else (
+        countGoodSyndromes(syndromes, s.n-s.f) >= s.n - s.f
+    ) 
+
+}
+
+function computeSyndrome(s: Node) : syndrome
+    requires s.state == Phase2;
+    requires 0 <= s.id < s.n;
+    requires s.n == |s.symbols| == |s.codeword|;
+    requires s.codeword[s.id] == s.symbols[s.id];
+{
+    computeSyndromeHelper(s.codeword, s.symbols)   
+}
+
+function computeSyndromeHelper(codeword: seq<nat>, symbols: seq<nat>) : syndrome
+    decreases codeword, symbols;
+    requires |codeword| == |symbols|
+{
+    if |codeword| == 0 then []
+    else [codeword[0] == symbols[0]] + computeSyndromeHelper(codeword[1..], symbols[1..])
+}
+
+/* Maps syndromes_seq to the number of syndromes in syndromes_seq that 
+* has #true bits >= thresh */
+function countGoodSyndromes(syndromes_seq: seq<syndrome>, thresh: int) : int
+    decreases syndromes_seq
+{
+    if |syndromes_seq| == 0 then 0 else
+    var x := countTrue(syndromes_seq[0]);
+    if x >= thresh then 1 + countGoodSyndromes(syndromes_seq[1..], thresh) else 
+    countGoodSyndromes(syndromes_seq[1..], thresh)
+}
+
+/* Maps syn to the number of True bits in syn */
+function countTrue(syn: syndrome) : int 
+    decreases syn
+{
+    if |syn| == 0 then 0 else (
+        if syn[0] then 1 + countTrue(syn[1..]) else countTrue(syn[1..])
+    )
+}
 }
